Allow comparing even more values in CAS by making things more consistent

theories/heap_lang/lang.v
@@ -68,9 +68,6 @@ Inductive expr :=
 
 Bind Scope expr_scope with expr.
 
-Notation NONE := (InjL (Lit LitUnit)) (only parsing).
-Notation SOME x := (InjR x) (only parsing).
-
 Fixpoint is_closed (X : list string) (e : expr) : bool :=
   match e with
   | Var x => bool_decide (x ∈ X)
@@ -99,9 +96,6 @@ Inductive val :=
 
 Bind Scope val_scope with val.
 
-Notation NONEV := (InjLV (LitV LitUnit)) (only parsing).
-Notation SOMEV x := (InjRV x) (only parsing).
-
 Fixpoint of_val (v : val) : expr :=
   match v with
   | RecV f x e => Rec f x e
@@ -120,6 +114,38 @@ Fixpoint to_val (e : expr) : option val :=
   | InjL e => InjLV <$> to_val e
   | InjR e => InjRV <$> to_val e
   | _ => None
+  end.
+
+(** We assume the following encoding of values to 64-bit words: The least 3
+significant bits of every word are a "tag", and we have 61 bits of payload,
+which is enough if all pointers are 8-byte-aligned (common on 64bit
+architectures). The tags have the following meaning:
+
+0: Payload is the data for a LitV (LitInt _).
+1: Payload is the data for a InjLV (LitV (LitInt _)).
+2: Payload is the data for a InjRV (LitV (LitInt _)).
+3: Payload is the data for a LitV (LitLoc _).
+4: Payload is the data for a InjLV (LitV (LitLoc _)).
+4: Payload is the data for a InjRV (LitV (LitLoc _)).
+6: Payload is one of the following finitely many values, which 61 bits are more
+   than enough to encode:
+   LitV LitUnit, InjLV (LitV LitUnit), InjRV (LitV LitUnit),
+   LitV (LitBool _), InjLV (LitV (LitBool _)), InjRV (LitV (LitBool _)).
+7: Value is boxed, i.e., payload is a pointer to some read-only memory area on
+   the heap which stores whether this is a RecV, PairV, InjLV or InjRV and the
+   relevant data for those cases. However, the boxed representation is never
+   used if any of the above representations could be used.
+
+Ignoring (as usual) the fact that we have to fit the infinite Z/loc into 61
+bits, this means every value is machine-word-sized and can hence be atomically
+read and written.  Also notice that the sets of boxed and unboxed values are
+disjoint. *)
+Definition val_is_unboxed (v : val) : Prop :=
+  match v with
+  | LitV _ => True
+  | InjLV (LitV _) => True
+  | InjRV (LitV _) => True
+  | _ => False
   end.
 
 (** The state: heaps of vals. *)
@@ -367,53 +393,13 @@ Definition bin_op_eval (op : bin_op) (v1 v2 : val) : option val :=
   | _, _ => None
   end.
 
-(** Return whether it is possible to use CAS to compare vl (current value) with
-v1 (netest value).
-
-We assume the following encoding of values to 64-bit words: The least 3
-significant bits of every word are a "tag", and we have 61 bits of payload,
-which is enough if all pointers are 8-byte-aligned (commong on 64bit
-architectures). The tags have the following meaning:
-
-0: Payload is one of the following finitely many values, which 61 bits are more
-   than enough to encode: LitV LitUnit, LitV (LitBool _), NONEV, SOMEV (LitV
-   LitUnit), SOMEV (LitV (LitBool _)).
-1: Payload is the data for a LitV (LitInt _).
-2: Payload is the data for a SOMEV (LitV (LitInt _)).
-3: Payload is the data for a LitV (LitLoc _).
-4: Payload is the data for a SOMEV (LitV (LitLoc _)).
-5: Value is boxed, i.e., payload is a pointer to some read-only memory area on
-   the heap which stores whether this is a RecV, PairV, InjLV or InjRV and the
-   relevant data for those cases. However, the boxed representation is never
-   used if any of the above representations could be used.
-6: Unused.
-7: Unused.
-
-Ignoring (as usual) the fact that we have to fit the infinite Z/loc into 61
-bits, this means every value is machine-word-sized and can hence be atomically
-read and written. It also justifies the comparisons allowed for CAS: Whenever
-[vals_cas_compare_safe vl v1] holds, equality of the one-word representation of
-[vl] and [v1] is equivalent to equality of the abstract value represented. This
-is clear for [LitV _ == LitV _] and [SOMEV (LitV _) == SOMEV (LitV _)] because
-none of these are boxed. For [NONEV == v], we can't actually atomically load and
-compare the data for boxed values, but that's okay because we only have to know
-if they are equal to [NONEV] which is distinct from all boxed values.
- *)
+(** CAS just compares the word-sized representation of the two values, it cannot
+look into boxed data.  This works out fine if at least one of the to-be-compared
+values is unboxed (exploiting the fact that an unboxed and a boxed value can
+never be equal because these are disjoint sets).  *)
 Definition vals_cas_compare_safe (vl v1 : val) : Prop :=
-  match vl, v1 with
-  (* We allow comparing literals with each other, also when wrapped in a SOMEV. *)
-  | LitV _, LitV _ => True
-  | SOMEV (LitV _), SOMEV (LitV _) => True
-  (* We allow comparing NONEV to anything. *)
-  | NONEV, _ => True
-  | _, NONEV => True
-  (* We don't allow comparing anything else. *)
-  | _, _ => False
-  end.
-(** Just a sanity check. *)
-Lemma vals_cas_compare_safe_sym vl v1 :
-  vals_cas_compare_safe vl v1 → vals_cas_compare_safe v1 vl.
-Proof. rewrite /vals_cas_compare_safe. repeat case_match; done. Qed.
+  val_is_unboxed vl ∨ val_is_unboxed v1.
+Arguments vals_cas_compare_safe !_ !_ /.
 
 Inductive head_step : expr → state → expr → state → list (expr) → Prop :=
   | BetaS f x e1 e2 v2 e' σ :
