tests/heap_lang.v
@@ -166,13 +166,6 @@ End printing_tests.
 Section error_tests.
   Context `{heapG Σ}.
 
-  Check "not_cas_compare_safe".
-  Lemma not_cas_compare_safe (l : loc) (v : val) :
-    l ↦ v -∗ WP CAS #l v v {{ _, True }}.
-  Proof.
-    iIntros "H↦". Fail wp_cas_suc.
-  Abort.
-
   Check "not_cas".
   Lemma not_cas :
     (WP #() {{ _, True }})%I.
